$$
\left\{
\begin{array}{lll}
X(t+\varDelta t)&=&X(t)+DX(t)\varDelta t+A(t)\sqrt{\frac{\hbar}{m}}\sqrt{\varDelta t} \\
Y(t+\varDelta t)&=&Y(t)+DY(t)\varDelta t+B(t)\sqrt{\frac{\hbar}{m}}\sqrt{\varDelta t} \\
Z(t+\varDelta t)&=&Z(t)+DZ(t)\varDelta t+C(t)\sqrt{\frac{\hbar}{m}}\sqrt{\varDelta t}
\end{array}
\right.
$$

$$
i h \frac{\partial \psi}{\partial t}=-\frac{\hbar^2}{2m}\varDelta\psi+\frac{e^2}{\sqrt{x^2+y^2+z^2}}\psi
$$

$$
\psi=\exp(R(x,y,z,t)+iS(x,y,z,t))
$$

$$
R={\rm Re}(\log\psi), S={\rm Im}(\log\psi)
$$

$$
\begin{array}{ll}
DX&=\frac{\hbar}{m}\left\{R_{x}+S_{x}\right\} \\
\\
DY&=\frac{\hbar}{m}\left\{R_{y}+S_{y}\right\} \\
\\
DZ&=\frac{\hbar}{m}\left\{R_{z}+S_{z}\right\} 
\end{array}
$$

$$
i \frac{\partial \psi}{\partial t}=-\frac{1}{2}\varDelta\psi+\frac{1}{\sqrt{x^2+y^2+z^2}}\psi
$$

$$
-\frac{1}{2}\varDelta+\frac{1}{\sqrt{x^2+y^2+z^2}}
$$

$$
E=-\frac{1}{2},-\frac{1}{8},-\frac{1}{18},\cdots,-\frac{1}{2n^{2}},\cdots
$$

$$
\psi=\frac{1}{4\sqrt{2\pi}}x\exp\left(-\frac{1}{2}\sqrt{x^2+y^{2}+z^{2}}+\frac{i}{8}t\right)
$$

$$
\left\{
\begin{array}{l}
X(t+\Delta t)=\displaystyle X(t)+\left(\frac{1}{X(t)}-\frac{1}{2}\frac{X(t)}{\sqrt{X(t)^{2}+Y(t)^{2}+Z(t)^{2}}}\right)\Delta t+A(t)\sqrt{\Delta t} \\
Y(t+\Delta t)=\displaystyle Y(t)-\frac{1}{2}\frac{Y(t)}{\sqrt{X(t)^{2}+Y(t)^{2}+Z(t)^{2}}}\Delta t+B(t)\sqrt{\Delta t} \\
Z(t+\Delta t)=\displaystyle Z(t)-\frac{1}{2}\frac{Z(t)}{\sqrt{X(t)^{2}+Y(t)^{2}+Z(t)^{2}}}\Delta t+C(t)\sqrt{\Delta t}
\end{array}
\right.
$$

